coq-osiris/examples/proofs/inversion.v
@@ -213,13 +213,14 @@ Section verification.
       handlerView γ Ys -∗
       deep_handler_spec ⊤ (ψ_yield l (iterView γ))
         (λ _ : outcome2 val exn, ∃ Xs : list A, iterView γ Xs ∗ ⌜complete Xs⌝)
-        (deep_eval_match
+        (λ o, deep_match_go
            ("__osiris_anonymous_arg" ~> VUnit;
             "yield" ~> yield;
             "Yield" ~> VLoc l;
             "iter" ~> iter;
             "__osiris_anonymous_arg" ~> iter;
             env)
+           o
            __branches3)
         ⊥ (RET h, isHead ⊥ h Ys).
     Proof.
