coq-osiris/theories/proofmode/setup.v
@@ -44,10 +44,9 @@ Arguments extendfs δ !fps !fvs.
 Arguments eval η !e /.
 Arguments evals η !es /.
 Arguments evalfs η !fes /.
-Arguments eval_match η !bs o.
-Arguments shallow_eval_match η !bs all_bs o.
-Arguments install_deep_eval_match η bs !o.
-Arguments deep_eval_match η !bs o /.
+Arguments shallow_match η o !bs all_bs.
+Arguments deep_match η !o bs.
+Arguments deep_match_go η o !bs /.
 Arguments eval_bindings η !bs /.
 Arguments eval_mexpr η !me /.
 Arguments eval_sitem ηδ !item /.
