coq-osiris/theories/stdlib/Stdlib.v
@@ -197,22 +197,22 @@ Definition compare_spec `{Encode A} (compare : val) (le : A → A → Prop) :=
           )).
 (* -------------------------------------------------------------------------- *)
 
-(* Lemma Stdlib__eq_spec : *)
-(*   decide_spec Stdlib__eq representable Logic.eq. (* same as Z.eq *) *)
-(* Proof. *)
-(*   intros x Hx. *)
-(*   pure_enter. simpl_eval. pure_enc_ret. *)
-(*   intros y Hy. *)
-(*   pure_enter. *)
-(*   eapply pure_eval_EOpEq_bool; try (pure_path); auto with encode. *)
-(* Qed. *)
+Lemma Stdlib__eq_spec :
+  decide_spec Stdlib__eq representable Logic.eq. (* same as Z.eq *)
+Proof.
+  intros x Hx.
+  pure_enter. simpl_eval. pure_ret.
+  intros y Hy.
+  pure_enter.
+  eapply pure_eval_EOpEq_bool; try (pure_path); auto with encode.
+Qed.
 
-(* Lemma Stdlib__ne_spec : *)
-(*   decide_spec Stdlib__ne representable (λ x y, x ≠ y). *)
-(* Proof. *)
-(*   intros x Hx. pure_enter. simpl_eval. pure_enc_ret. intros y Hy. pure_enter. *)
-(*   eapply pure_eval_EOpNe_bool; try (pure_path); auto. *)
-(* Qed. *)
+Lemma Stdlib__ne_spec :
+  decide_spec Stdlib__ne representable (λ x y, x ≠ y).
+Proof.
+  intros x Hx. pure_enter. simpl_eval. pure_ret. intros y Hy. pure_enter.
+  eapply pure_eval_EOpNe_bool; try (pure_path); auto.
+Qed.
 
 (* Lemma Stdlib__lt_spec : *)
 (*   decide_spec Stdlib__lt representable Z.lt. *)
