coq-osiris/theories/test/wp_test.v
@@ -9,7 +9,7 @@ From osiris.proofmode Require Import ewp_tactics.
 
 Context `{!osirisGS Σ} `{protocol_wf Σ}.
 
-Local Transparent eval eval_mexpr eval_match eval_sitem eval_sitems
+Local Transparent eval eval_mexpr eval_sitem eval_sitems
   eval_bindings evals extend extends encode.
 
 (* ---------------------------------------------------------------------------*)
